ChecksumLog.v: rep function for a list of hashes, updated recover_ok proof to match

src/ChecksumLog.v
@@ -25,13 +25,27 @@ Definition hash_block : addr := $2.
 
 Definition hash2 (a b : word valulen) := hash_to_valu (hash_fwd (Word.combine a b)).
 
+Definition hash2_rep a b v :=
+  v = hash2 a b /\
+  hash_inv (hash_fwd (Word.combine a b)) = existT _ _ (Word.combine a b).
+
+Fixpoint list_hash2_rep lhv lab :=
+  match lhv with
+  | nil => True
+  | hv :: lhv' => match lab with
+    | nil => False
+    | (a, b) :: lab' => hash2_rep a b hv /\ list_hash2_rep lhv' lab'
+    end
+  end.
+
 (* block1 and block2 are synced, hash_block has some valid hash *)
 Definition any_hash_rep a b a' b' (d : @mem addr (@weq addrlen) valuset) :
     @pred addr (@weq addrlen) valuset :=
-  [[ (block1 |-> (a, nil) *
-   block2 |-> (b, nil) *
-   hash_block |-> (hash2 a' b', nil))%pred d ]] *
-  [[ hash_inv (hash_fwd (Word.combine a' b')) = existT _ _ (Word.combine a' b') ]].
+  (exists hv,
+    [[ (block1 |-> (a, nil) *
+     block2 |-> (b, nil) *
+     hash_block |-> (hv, nil))%pred d ]] *
+    [[ hash2_rep a' b' hv ]])%pred.
 
 (* hash_block has the valid hash of block1 and block2 values *)
 Definition rep a b (d : @mem addr (@weq addrlen) valuset) :
@@ -42,12 +56,14 @@ Definition rep a b (d : @mem addr (@weq addrlen) valuset) :
   - block1 and block2 can be anything
   - hash_block points to a valid hash
   - hash_block can have unsynced values (how to state cleanly that these are also valid hashes? *)
-Definition hash_crep a b l :
+Definition hash_crep a b l lhv :
     @pred addr (@weq addrlen) valuset :=
-  (block1 |->? *
+  (exists hv,
+   block1 |->? *
    block2 |->? *
-   hash_block |-> (hash2 a b, l)) *
-  [[ hash_inv (hash_fwd (Word.combine a b)) = existT _ _ (Word.combine a b) ]]%pred.
+   hash_block |-> (hv, l) *
+   [[ list_hash2_rep (hv :: l) ((a, b) :: lhv) ]])%pred.
+
 
 (* After a crash, hash_block is one of:
   - hash of old values
@@ -55,9 +71,9 @@ Definition hash_crep a b l :
   - hash of new values and synced *)
 Definition crep a b a' b' :
     @pred addr (@weq addrlen) valuset :=
-  (hash_crep a b nil \/
-  hash_crep a' b' (hash2 a b :: nil) * [[ hash_inv (hash_fwd (Word.combine a b)) = existT _ _ (Word.combine a b) ]] \/
-  hash_crep a' b' nil).
+  (hash_crep a b nil nil \/
+    hash_crep a' b' ((hash2 a b) :: nil) ((a, b) :: nil) \/
+    hash_crep a' b' nil nil).
 
 
 (* Example "log" implementation using checksums *)
@@ -105,9 +121,7 @@ Theorem put_ok : forall cs d1 d2,
       [[ (crep d1_old' d2_old' d1 d2)%pred d' ]]
   >} put cs d1 d2.
 Proof.
-  unfold put, any_hash_rep, rep, crep, hash_crep.
-  step.
-
+  unfold put, rep, any_hash_rep, crep, hash_crep, list_hash2_rep, hash2_rep.
   step.
   step.
   step.
@@ -115,7 +129,7 @@ Proof.
   step.
   step.
   step.
-  unfold any_hash_rep. cancel.
+  step.
 
   Grab Existential Variables.
   all: eauto.
@@ -147,26 +161,23 @@ Qed.
 (* block1 and block2 get some value, and hash_block points to a valid hash of  *)
 Definition after_crash_pred v1 v2 :
     @pred addr (@weq addrlen) valuset :=
-  (exists a b, 
+  (exists a b hv,
       block1 |-> (a, nil) *
       block2 |-> (b, nil) *
-      hash_block |-> (hash2 v1 v2, nil) *
-    [[ hash_inv (hash_fwd (Word.combine v1 v2)) = existT _ _ (Word.combine v1 v2) ]])%pred.
+      hash_block |-> (hv, nil) *
+    [[ hash2_rep v1 v2 hv ]])%pred.
 
 Lemma crash_xform_would_recover_either_pred : forall v1 v2 v1' v2',
   crash_xform (crep v1 v2 v1' v2') =p=>
     after_crash_pred v1 v2 \/
     after_crash_pred v1' v2'.
 Proof.
-  unfold crep, hash_crep, after_crash_pred.
+  unfold crep, hash_crep, list_hash2_rep, after_crash_pred.
   intros.
   autorewrite with crash_xform.
   cancel.
 
-  autorewrite with crash_xform. cancel.
-  autorewrite with crash_xform. cancel.
-  autorewrite with crash_xform. cancel.
-  autorewrite with crash_xform. cancel.
+  all: repeat (autorewrite with crash_xform; cancel; autorewrite with crash_xform; cancel).
 Qed.
 
 Hint Rewrite crash_xform_would_recover_either_pred : crash_xform.
@@ -213,22 +224,27 @@ Proof.
     step.
     step.
     step.
-    unfold hash2 in *.
-    apply hash_to_valu_inj in H8.
+    unfold hash2_rep, hash2 in *.
+    destruct H5.
+
     assert (Hheq: d1_old = a /\ d2_old = b).
-      rewrite H8 in H5.
-      rewrite H5 in H11.
-      pose proof (eq_sigT_snd H11).
+      apply hash_to_valu_inj in H0.
+      rewrite H0 in H11.
+      rewrite H11 in H3.
+      pose proof (eq_sigT_snd H3).
       autorewrite with core in *.
-      apply combine_inj in H0.
+      apply combine_inj in H5.
+      destruct H5.
       auto.
-    unfold any_hash_rep.
+    unfold any_hash_rep, hash2_rep.
     cancel.
 
-    step. unfold any_hash_rep. cancel.
+    step. unfold any_hash_rep, hash2_rep, hash2 in *. cancel.
     step.
-    cancel. instantiate (1:=d'). cancel.
-    all: cancel; try (unfold crep, hash_crep in *; instantiate (1:=d); cancel).
+    cancel.
+    all: cancel; try (unfold crep, hash_crep, list_hash2_rep, hash2_rep in *;
+      instantiate (1:=d);
+      cancel).
 
   - cancel.
     step.
@@ -236,21 +252,27 @@ Proof.
     step.
     step.
     step.
+    unfold hash2_rep, hash2 in *.
+    destruct H5.
+
     assert (Hheq: d1 = a /\ d2 = b).
-      apply hash_to_valu_inj in H8.
-      rewrite H8 in H5.
-      rewrite H5 in H11.
-      pose proof (eq_sigT_snd H11).
+      apply hash_to_valu_inj in H0.
+      rewrite H0 in H11.
+      rewrite H11 in H3.
+      pose proof (eq_sigT_snd H3).
       autorewrite with core in *.
-      apply combine_inj in H0.
+      apply combine_inj in H5.
+      destruct H5.
       auto.
-    unfold any_hash_rep.
+    unfold any_hash_rep, hash2_rep.
     cancel.
 
-    step. unfold any_hash_rep. cancel.
+    step. unfold any_hash_rep, hash2_rep, hash2 in *. cancel.
     step.
-    cancel. instantiate (1:=d'). cancel.
-    all: cancel; try (unfold crep, hash_crep in *; instantiate (1:=d); cancel).
+    cancel.
+    all: cancel; try (unfold crep, hash_crep, list_hash2_rep, hash2_rep in *;
+      instantiate (1:=d);
+      cancel).
 
   Grab Existential Variables.
   all: eauto.
